WIP -- weird... ?

theories/Semantics.v
@@ -5,6 +5,7 @@ Inductive sort: Type :=
 | angelic
 | demonic
 | final
+| vis
 .
 
 Record semantics : Type := Semantics_gen {
@@ -12,4 +13,7 @@ Record semantics : Type := Semantics_gen {
   step : state -> option event -> state -> Prop;
   initial_state: state;
   state_sort: state -> sort;
+  wf_vis: forall st0 (VIS: state_sort st0 = vis), exists ! ev st1, step st0 (Some ev) st1;
+  wf_angelic: forall st0 ev st1 (VIS: state_sort st0 = angelic) (STEP: step st0 ev st1), ev = None;
+  wf_demonic: forall st0 ev st1 (VIS: state_sort st0 = demonic) (STEP: step st0 ev st1), ev = None;
 }.
