theories/SimSingle.v
@@ -105,7 +105,7 @@ Proof.
   remember [e] as tmp in STAR. revert Heqtmp.
   induction STAR; ii; ss. punfold SPIN. rr in STEP; des. inv SPIN; ii; rewrite PROP in *; ss.
   destruct ev, evs; ss; clarify.
-  - exploit STEP; eauto. i; des; ss.
+  - exploit wf_angelic; et. i; ss.
   - exploit STEP; eauto. i; des; ss. pclearbot. eapply IHSTAR; eauto.
 Qed.
 
@@ -123,6 +123,19 @@ Proof.
     exploit STEP; eauto. i; des. pclearbot. eapply IHSTAR; ss. }
 Qed.
 
+Lemma spin_astep
+      L st0 ev st1
+      (SRT: L.(state_sort) st0 = angelic)
+      (STEP: _.(step) st0 ev st1)
+      (SPIN: Beh.state_spin _ st0)
+  :
+    <<SPIN: Beh.state_spin _ st1>>
+.
+Proof.
+  exploit wf_angelic; et. i; clarify.
+  punfold SPIN. inv SPIN; rewrite SRT in *; ss.
+  exploit STEP0; et. i; des. pclearbot. et.
+Qed.
 
 
 
@@ -133,23 +146,31 @@ Section SIM.
   Variable ord: idx -> idx -> Prop.
 
   Variant _sim sim (i0: idx) (st_src0: L0.(state)) (st_tgt0: L1.(state)): Prop :=
-  | sim_event
-      (SRT: _.(state_sort) st_src0 = demonic)
-      (SRT: _.(state_sort) st_tgt0 = demonic)
-      (SAFE: exists ev st_tgt1, _.(step) st_tgt0 (Some ev) st_tgt1)
-      (SIM: forall ev st_tgt1
-          (STEP: _.(step) st_tgt0 ev st_tgt1)
-        ,
-          exists i1 st_src1, <<EVENT: is_some ev>> /\
-                             <<STEP: _.(step) st_src0 ev st_src1>> /\
-                             <<SIM: sim i1 st_src1 st_tgt1>>)
+  | sim_fin
+      (SRT: _.(state_sort) st_src0 = final)
+      (SRT: _.(state_sort) st_tgt0 = final)
+    :
+      _sim sim i0 st_src0 st_tgt0
+
+  | sim_vis
+      (SRT: _.(state_sort) st_src0 = vis)
+      (SRT: _.(state_sort) st_tgt0 = vis)
+      ev st_src1 st_tgt1
+      (STEP: _.(step) st_src0 ev st_src1)
+      (STEP: _.(step) st_tgt0 ev st_tgt1)
+      (* (SIM: forall ev st_tgt1 *)
+      (*     (STEP: _.(step) st_tgt0 ev st_tgt1) *)
+      (*   , *)
+      (*     exists i1 st_src1, <<EVENT: is_some ev>> /\ *)
+      (*                        <<STEP: _.(step) st_src0 ev st_src1>> /\ *)
+      (*                        <<SIM: sim i1 st_src1 st_tgt1>>) *)
     :
       _sim sim i0 st_src0 st_tgt0
 
 
   | sim_demonic_src
       (SRT: _.(state_sort) st_src0 = demonic)
-      (FIN: _.(state_sort) st_src0 = final <-> _.(state_sort) st_tgt0 = final)
+      (* (FIN: _.(state_sort) st_src0 = final <-> _.(state_sort) st_tgt0 = final) *)
       (SIM: exists st_src1
           (STEP: _.(step) st_src0 None st_src1)
         ,
@@ -158,7 +179,7 @@ Section SIM.
       _sim sim i0 st_src0 st_tgt0
   | sim_demonic_tgt
       (SRT: _.(state_sort) st_tgt0 = demonic)
-      (FIN: _.(state_sort) st_src0 = final <-> _.(state_sort) st_tgt0 = final)
+      (* (FIN: _.(state_sort) st_src0 = final <-> _.(state_sort) st_tgt0 = final) *)
       (SIM: forall st_tgt1
           (STEP: _.(step) st_tgt0 None st_tgt1)
         ,
@@ -167,7 +188,7 @@ Section SIM.
       _sim sim i0 st_src0 st_tgt0
   | sim_angelic_src
       (SRT: _.(state_sort) st_src0 = angelic)
-      (FIN: _.(state_sort) st_src0 = final <-> _.(state_sort) st_tgt0 = final)
+      (* (FIN: _.(state_sort) st_src0 = final <-> _.(state_sort) st_tgt0 = final) *)
       (SIM: forall st_src1
           (STEP: _.(step) st_src0 None st_src1)
         ,
@@ -176,7 +197,7 @@ Section SIM.
       _sim sim i0 st_src0 st_tgt0
   | sim_angelic_tgt
       (SRT: _.(state_sort) st_tgt0 = angelic)
-      (FIN: _.(state_sort) st_src0 = final <-> _.(state_sort) st_tgt0 = final)
+      (* (FIN: _.(state_sort) st_src0 = final <-> _.(state_sort) st_tgt0 = final) *)
       (SIM: exists st_tgt1
           (STEP: _.(step) st_tgt0 None st_tgt1)
         ,
@@ -188,45 +209,41 @@ Section SIM.
   | sim_demonic_both
       (SRT: _.(state_sort) st_src0 = demonic)
       (SRT: _.(state_sort) st_tgt0 = demonic)
-      (FIN: _.(state_sort) st_src0 = final <-> _.(state_sort) st_tgt0 = final)
       (SIM: forall st_tgt1
           (STEP: _.(step) st_tgt0 None st_tgt1)
         ,
-          exists st_src1, <<STEP: _.(step) st_src0 None st_src1>> /\
-                                  <<SIM: exists i1, sim i1 st_src0 st_tgt1>>)
+          exists st_src1 (STEP: _.(step) st_src0 None st_src1),
+            <<SIM: exists i1, sim i1 st_src1 st_tgt1>>)
     :
       _sim sim i0 st_src0 st_tgt0
   | sim_angelic_both
       (SRT: _.(state_sort) st_src0 = angelic)
       (SRT: _.(state_sort) st_tgt0 = angelic)
-      (FIN: _.(state_sort) st_src0 = final <-> _.(state_sort) st_tgt0 = final)
       (SIM: forall st_src1
           (STEP: _.(step) st_src0 None st_src1)
         ,
-          exists st_tgt1, <<STEP: _.(step) st_tgt0 None st_tgt1>> /\
-                                  <<SIM: exists i1, sim i1 st_src0 st_tgt1>>)
+          exists st_tgt1 (STEP: _.(step) st_tgt0 None st_tgt1),
+            <<SIM: exists i1, sim i1 st_src1 st_tgt1>>)
     :
       _sim sim i0 st_src0 st_tgt0
   | sim_demonic_angelic
       (SRT: _.(state_sort) st_src0 = demonic)
       (SRT: _.(state_sort) st_tgt0 = angelic)
-      (FIN: _.(state_sort) st_src0 = final <-> _.(state_sort) st_tgt0 = final)
       (SIM: exists st_tgt1
           (STEP: _.(step) st_tgt0 None st_tgt1)
         ,
-          exists st_src1, <<STEP: _.(step) st_src0 None st_src1>> /\
-                                     <<SIM: exists i1, sim i1 st_src0 st_tgt1>>)
+          exists st_src1 (STEP: _.(step) st_src0 None st_src1),
+            <<SIM: exists i1, sim i1 st_src1 st_tgt1>>)
     :
       _sim sim i0 st_src0 st_tgt0
   | sim_angelic_demonic
       (SRT: _.(state_sort) st_src0 = angelic)
       (SRT: _.(state_sort) st_tgt0 = demonic)
-      (FIN: _.(state_sort) st_src0 = final <-> _.(state_sort) st_tgt0 = final)
       (SIM: forall st_src1
           (STEP: _.(step) st_src0 None st_src1)
         ,
-          forall st_tgt1, <<STEP: _.(step) st_tgt0 None st_tgt1>> /\
-                                  <<SIM: exists i1, sim i1 st_src0 st_tgt1>>)
+          forall st_tgt1 (STEP: _.(step) st_tgt0 None st_tgt1),
+            <<SIM: exists i1, sim i1 st_src1 st_tgt1>>)
     :
       _sim sim i0 st_src0 st_tgt0
 
@@ -303,17 +320,18 @@ Section SIM.
 
   Lemma sim_mon: monotone3 _sim.
   Proof.
-    ii. inv IN; try (by econs; eauto).
+    ii. inv IN.
 
-    - econs 1; et. i. exploit SIM; et. i; des. esplits; et.
-    - econs 2; et. des. esplits; et.
-    - econs 3; et. i. exploit SIM; et. i; des. esplits; et.
+    - econs 1; et.
+    - econs 2; et.
+    - econs 3; et. des. esplits; et.
     - econs 4; et. i. exploit SIM; et. i; des. esplits; et.
-    - econs 5; et. des. esplits; et.
-    - econs 6; et. i. exploit SIM; et. i; des. esplits; et.
+    - econs 5; et. i. exploit SIM; et. i; des. esplits; et.
+    - econs 6; et. des. esplits; et.
     - econs 7; et. i. exploit SIM; et. i; des. esplits; et.
-    - econs 8; et. des. esplits; et.
-    - econs 9; et. i. exploit SIM; et. i; des. esplits; et.
+    - econs 8; et. i. exploit SIM; et. i; des. esplits; et.
+    - econs 9; et. des. esplits; et.
+    - econs 10; et. i. exploit SIM; et. i; des. esplits; et.
   Qed.
 
   Hint Constructors _sim.
@@ -345,43 +363,53 @@ Section SIM.
     rename x into i0. rename H into IH.
 
     punfold SIM. inv SIM.
-    - des. exfalso. punfold SPIN. inv SPIN.
-      + exploit STEP; et. i; des. ss.
-      + des. clarify. exploit SIM0; et. i; des. ss.
-    - des. pc SIM. gstep. econs 2; et. esplits; et. gbase. et.
-    - punfold SPIN. inv SPIN; try rewrite SRT in *; ss. des; clarify.
-      pc TL. exploit SIM0; et. i; des. pc SIM. eapply IH; et.
-    - punfold SPIN. inv SPIN; ss.
+    - (** final **)
+      des. exfalso. punfold SPIN. inv SPIN; rewrite SRT1 in *; ss.
+    - (** vis **)
+      des. exfalso. punfold SPIN. inv SPIN; rewrite SRT1 in *; ss.
+    - (** dsrc **)
+      des. pc SIM. gstep. econs 2; et. esplits; et. gbase. et.
+    - (** dtgt **)
+      punfold SPIN. inv SPIN; try rewrite SRT in *; ss. des; clarify.
+      pc TL. exploit wf_demonic; et; i; clarify.
+      exploit SIM0; et. i; des. pc SIM. eapply IH; et.
+    - (** asrc **)
+      punfold SPIN. inv SPIN; ss.
       + gstep. econs 1; et. ii.
-        TTTTTTTTTTTTTTTTTTTTTTTTTTTTTT
-        exploit SIM0; et.
-        exploit STEP; et. i; des. clarify. pc TL.
-        destruct (classic (exists ev st_tgt1, _.(step) st_tgt0 ev st_tgt1)).
-        * des. exploit STEP; et. i; des. clarify. pc TL.
-      pc TL. exploit SIM0; et. i; des. pc SIM. eapply IH; et.
-      gstep. econs 2; et.
-      
-      pc SIM. gstep. econs 2; et. esplits; et.
-    (* - eapply spin_nofinal in SPIN; ss. *)
-    - punfold SPIN. inv SPIN; rewrite DEM in *; ss. des. clarify.
-      rename st1 into st_tgt1.
-      exploit STEPSIM; eauto. pclearbot. i; des; rr in SIM; des; ss; cycle 1.
-      { clarify. eapply IH; eauto. }
-      rr in STEP; des.
-      gstep. econs 2; eauto. esplits; eauto. gbase. eapply CIH; eauto.
-    - gstep. econs; eauto. ii. exploit STEPSIM; eauto. i; des; ss; clarify; rr in SIM; des; ss; cycle 1.
-      { rename st1 into st_src1. esplits; eauto. exploit IH; eauto.
-        ii. eapply gpaco1_mon_gen; eauto. { eapply Beh.state_spin_mon. } ii; ss.
-      }
-      rr in STEP0; des.
-      punfold SPIN. inv SPIN; ss; rewrite PROP in *; ss.
-      exploit STEP0; eauto. i; des. clarify. rr in TL; des; ss. clarify.
-      rename st1 into st_src1. esplits; eauto.
-      gbase. eapply CIH; eauto.
+        exploit L0.(wf_angelic); et. i; clarify. esplits; et.
+        exploit SIM0; et. i; des. pc SIM.
+        gbase. eapply CIH; eauto.
+      + des; clarify. rename st1 into st_tgt1.
+        exploit wf_demonic; et; i; clarify.
+        gstep. econs; et. ii. exploit wf_angelic; et; i; clarify.
+        pc TL. exploit SIM0; et. i; des. pc SIM.
+        (* gbase. eapply CIH; et. pfold; econs 2; et. esplits; et. *)
+        eapply gpaco1_mon. { eapply IH; et. pfold; econs 2; et. esplits; et. } { ss. } { ss. }
+    - (** atgt **)
+      des. pc SIM. eapply IH; eauto. eapply spin_astep; et.
+    - (** dd **)
+      punfold SPIN. inv SPIN; rewrite SRT0 in *; ss. des.
+      exploit wf_demonic; et; i; clarify. pc TL.
+      exploit SIM0; et. i; des. pc SIM.
+      gstep. econs 2; et. esplits; et. gbase. eapply CIH; et.
+    - (** aa **)
+      punfold SPIN. inv SPIN; rewrite SRT0 in *; ss. des.
+      gstep. econs; et. ii.
+      exploit L0.(wf_angelic); et; i; clarify.
+      exploit SIM0; et. i; des. pc SIM.
+      gbase. eapply CIH; et. eapply spin_astep; et.
+    - (** da **)
+      des. pc SIM. gstep. econs 2; et. esplits; et. gbase. eapply CIH; et. eapply spin_astep; et.
+    - (** ad **)
+      gstep. econs 1; et. ii.
+      exploit L0.(wf_angelic); et; i; clarify.
+      punfold SPIN. inv SPIN; rewrite SRT0 in *; ss. des; clarify. pc TL.
+      exploit (wf_demonic); et; i; clarify.
+      exploit SIM0; et. i; des. pc x.
+      gbase. eapply CIH; et.
   Qed.
 
   Lemma adequacy_final
-        (WF: well_founded ord)
         i0 st_src0 st_tgt0
         (SIM: sim i0 st_src0 st_tgt0)
         (FIN: Beh.of_state L1 st_tgt0 Tr.done)
@@ -389,21 +417,121 @@ Section SIM.
       <<FIN: Beh.of_state L0 st_src0 Tr.done>>
   .
   Proof.
-    punfold SIM; inv SIM.
-    - punfold FIN.
-      generalize dependent st_src0.
-      generalize dependent i0.
-      dependent induction FIN using Beh.of_state_ind; ii; try rewrite DEM in *; ss;
-        rename st0 into st_tgt0.
-      rr in STEP. des. clarify. rename st1 into st_tgt1.
-      exploit STEPSIM; eauto. i; des.
-      + rr in STEP; des; ss. rr in SIM; des; ss. exploit IH; ss; eauto.
-      +
-      apply FIN0 in FINAL.
+    revert_until WF.
+    pcofix CIH. i.
+    revert_until i0. pattern i0. eapply well_founded_ind; eauto. clear i0. i.
+    rename x into i0. rename H into IH.
 
-      inv FIN; try rewrite DEM in *; ss.
-      rr in STEP. des. clarify. inv TL.
-      apply FIN0 in FINAL.
+    punfold FIN. generalize dependent st_src0.
+    generalize dependent i0.
+    dependent induction FIN using Beh.of_state_ind; ii; ss.
+    - (** final **)
+      punfold SIM; inv SIM; try rewrite H in *; ss.
+      + pfold. econs; eauto.
+      + des. pfold. econs 6; eauto. rr. esplits; et. pc SIM. exploit IH; et. intro A. punfold A.
+      + pfold. econs 7; eauto. ii. exploit wf_angelic; et. i; clarify.
+        exploit SIM0; et. i; des. pc SIM. esplits; et.
+        exploit IH; et. intro A. punfold A.
+    - (** demonic **)
+      rr in STEP. des. clarify.
+      punfold SIM; inv SIM; try rewrite DEM in *; ss.
+      + des. pfold. econs 6; eauto. rr. esplits; et. pc SIM.
+        exploit IH; et. { eapply Beh.beh_dstep; et. } intro A. punfold A.
+      + exploit SIM0; et. i; des. pc SIM. exploit IH; et.
+      + pfold. econs 7; eauto. ii. exploit wf_angelic; et. i; clarify.
+        exploit SIM0; et. i; des. pc SIM. esplits; et.
+        exploit IH; et. { eapply Beh.beh_dstep; et. } intro A. punfold A.
+      + exploit SIM0; et. i; des. pc SIM.
+        pfold. econs 6; et. rr. esplits; et.
+        exploit IH0; revgoals.
+        { intro A. punfold A. }
+        { et. }
+        { specialize (IH0 (eq_refl _)). specialize (IH0 i1).
+        }
+        et. { eapply Beh.beh_dstep; et. } intro A. punfold A.
+        pfold. econs 6; et. rr. esplits; et.
+        exploit SIM0; et. i; des. pc SIM. exploit IH; et.
+      + exploit SIM0; et. i; des. pc SIM. exploit IH; et.
+      +
+        pfold. econs 7; eauto.
+        exploit IH; et. { pfold. econs 6; et. rr. esplits; et. } intro A. punfold A.
+      pfold. econs 6; eauto.
+      exploit IH; et.
+    - (** angelic **)
+    punfold SIM; inv SIM.
+    - (** final **)
+      punfold FIN.
+    - (** vis **)
+      punfold FIN. inv FIN; rewrite SRT0 in *; ss.
+    - (** dsrc **)
+      des. pc SIM. pfold. econs 6; eauto. rr. esplits; et. exploit IH; et. intro A. punfold A.
+    - (** dtgt **)
+      punfold FIN. inv FIN; rewrite SRT in *; ss. rr in STEP. des; clarify.
+      exploit SIM0; et. i; des. pc SIM.
+      eapply IH; et.
+    - (** asrc **)
+      pfold. econs 7; et. ii. exploit wf_angelic; et. i; clarify. esplits; et.
+      exploit SIM0; et. i; des. pc SIM. exploit IH; et. intro A. punfold A.
+    - (** atgt **)
+      des. pc SIM. exploit IH; et. eapply Beh.beh_astep; et.
+    - (** dd **)
+      punfold FIN. inv FIN; try rewrite SRT0 in *; ss. rr in STEP. des; clarify.
+      exploit SIM0; et. i; des. pc SIM.
+      pfold. econs 6; et. rr. esplits; et.
+    - (** aa **)
+    - (** da **)
+    - (** ad **)
+  Qed.
+
+  Lemma adequacy_final
+        i0 st_src0 st_tgt0
+        (SIM: sim i0 st_src0 st_tgt0)
+        (FIN: Beh.of_state L1 st_tgt0 Tr.done)
+    :
+      <<FIN: Beh.of_state L0 st_src0 Tr.done>>
+  .
+  Proof.
+    revert_until WF.
+    (* ginit. *)
+    (* { i. eapply cpn2_wcompat; eauto. eapply Beh.of_state_mon. } *)
+    (* gcofix CIH. i. *)
+    pcofix CIH. i.
+    revert_until i0. pattern i0. eapply well_founded_ind; eauto. clear i0. i.
+    rename x into i0. rename H into IH.
+
+    punfold SIM; inv SIM.
+    (* - (** final **) *)
+    (* - (** vis **) *)
+    (* - (** dsrc **) *)
+    (* - (** dtgt **) *)
+    (* - (** asrc **) *)
+    (* - (** atgt **) *)
+    (* - (** dd **) *)
+    (* - (** aa **) *)
+    (* - (** da **) *)
+    (* - (** ad **) *)
+    - (** final **)
+      punfold FIN.
+    - (** vis **)
+      punfold FIN. inv FIN; rewrite SRT0 in *; ss.
+    - (** dsrc **)
+      des. pc SIM. pfold. econs 6; eauto. rr. esplits; et. exploit IH; et. intro A. punfold A.
+    - (** dtgt **)
+      punfold FIN. inv FIN; rewrite SRT in *; ss. rr in STEP. des; clarify.
+      exploit SIM0; et. i; des. pc SIM.
+      eapply IH; et.
+    - (** asrc **)
+      pfold. econs 7; et. ii. exploit wf_angelic; et. i; clarify. esplits; et.
+      exploit SIM0; et. i; des. pc SIM. exploit IH; et. intro A. punfold A.
+    - (** atgt **)
+      des. pc SIM. exploit IH; et. eapply Beh.beh_astep; et.
+    - (** dd **)
+      punfold FIN. inv FIN; try rewrite SRT0 in *; ss. rr in STEP. des; clarify.
+      exploit SIM0; et. i; des. pc SIM.
+      pfold. econs 6; et. rr. esplits; et.
+    - (** aa **)
+    - (** da **)
+    - (** ad **)
   Qed.
 
   (* Record semantics_wf (L: semantics): Prop := mk_swf { *)
